src/Correctness/ForwardingCorrect.v
@@ -20,37 +20,19 @@ Context {node_id_edge_set : map.map node_id node_id_set} {node_id_edge_set_ok : 
 Notation node_graph := (@ComputableGraph.ComputableGraph node_id node_id_set node_id_edge_set).
 Notation cg_edge := (@ComputableGraph.cg_edge node_id node_id_set node_id_edge_set).
 
-Notation destination := (@DistributedHardwareProgram.destination node_id).
-Context {forwarding_table : map.map rel_id (list destination)}
+Context {forwarding_table : map.map rel_id (list node_id)}
         {forwarding_table_ok : map.ok forwarding_table}.
 Context {node_ftable_map : map.map node_id forwarding_table}
         {node_ftable_map_ok : map.ok node_ftable_map}.
 
 Notation node_info := (@DistributedHardwareProgram.node_info node_id forwarding_table).
-Notation get_node_ftable node ftables := (get_or_default ftables node).
-
-(* the [DestEdge] targets among a destination list *)
-Definition dest_edges (ds : list destination) : list node_id :=
-  flat_map (fun d => match d with
-                     | DistributedHardwareProgram.DestEdge n => [n]
-                     | DistributedHardwareProgram.DestTrie _ => [] end) ds.
-
-(* [x] is a [DestEdge] target of [ds] iff [DestEdge x] is literally in [ds]. *)
-Lemma In_dest_edges (x : node_id) (ds : list destination) :
-  In x (dest_edges ds) <-> In (DistributedHardwareProgram.DestEdge x) ds.
-Proof.
-  unfold dest_edges. rewrite in_flat_map. split.
-  - intros [d [Hin Hx]]. destruct d as [n|t]; cbn in Hx; [|destruct Hx].
-    destruct Hx as [<-|[]]. exact Hin.
-  - intros Hin. exists (DistributedHardwareProgram.DestEdge x). split; [exact Hin | left; reflexivity].
-Qed.
 
 (* the forwarding edges node [node] has for relation [rel] in [ftables] *)
-Definition node_rel_dests (ftables : node_ftable_map) (node : node_id) (rel : rel_id) : list destination :=
-  match map.get (get_node_ftable node ftables) rel with Some ds => ds | None => [] end.
+Definition node_rel_dests (ftables : node_ftable_map) (node : node_id) (rel : rel_id) : list node_id :=
+  get_or_default (get_or_default ftables node) rel.
 
 Definition has_fwd_edge (ftables : node_ftable_map) (node : node_id) (rel : rel_id) (m : node_id) : Prop :=
-  In m (dest_edges (node_rel_dests ftables node rel)).
+  In m (node_rel_dests ftables node rel).
 
 (*============================================================================*)
 (*  Soundness: every forwarding edge is a real graph edge                      *)
@@ -59,20 +41,6 @@ Definition has_fwd_edge (ftables : node_ftable_map) (node : node_id) (rel : rel_
 (* the table is *edge-sound* when every forwarding edge it records is a real graph edge *)
 Definition ftable_edges_sound (g : node_graph) (ftables : node_ftable_map) : Prop :=
   forall node rel m, has_fwd_edge ftables node rel m -> cg_edge g node m.
-
-
-Context {internode_forwarding_table : map.map rel_id (list node_id)}
-        {internode_forwarding_table_ok : map.ok internode_forwarding_table}.
-Context {internode_forwarding_tables : map.map node_id internode_forwarding_table}
-        {internode_forwarding_tables_ok : map.ok internode_forwarding_tables}.
-
-Notation ftables_in_graphb := (@DistributedDatalogToHardwareCompiler.ftables_in_graphb node_id node_id_set node_id_edge_set internode_forwarding_table internode_forwarding_tables).
-Notation graph_of_ftables_at_rel := (@DistributedDatalogToHardwareCompiler.graph_of_ftables_at_rel node_id node_id_set node_id_edge_set internode_forwarding_table internode_forwarding_tables).
-Notation compute_forwarding_table := (@DistributedDatalogToHardwareCompiler.compute_forwarding_table node_id forwarding_table node_ftable_map internode_forwarding_table internode_forwarding_tables).
-
-(* the hops the external table records for [R] at [n]: the single notion both the induced graph
-   and the computed table are built from. *)
-Notation next_hops ftables n R := (get_or_default (get_or_default ftables n) R).
 
 Lemma get_map_values {K V1 V2 : Type} {keqb : Eqb K} {keqb_ok : Eqb_ok keqb}
     {M1 : map.map K V1} {M1ok : map.ok M1} {M2 : map.map K V2} {M2ok : map.ok M2}
@@ -96,89 +64,14 @@ Proof.
     + rewrite IH. split; [tauto | intros [Heq|H]; [congruence | exact H]].
 Qed.
 
-Lemma dest_edges_app (A B : list destination) :
-  dest_edges (A ++ B) = dest_edges A ++ dest_edges B.
-Proof. unfold dest_edges. apply flat_map_app. Qed.
-
-Lemma dest_edges_map_edge (l : list node_id) :
-  dest_edges (List.map DistributedHardwareProgram.DestEdge l) = l.
-Proof. unfold dest_edges. induction l as [|x l IH]; cbn; congruence. Qed.
-
-(* [trie_ftable] only ever stores [DestTrie]s, so it contributes no forwarding edge *)
-Lemma trie_ftable_no_edges' (tries : list trie) (R : rel_id) :
-  dest_edges (get_or_default (DistributedDatalogToHardwareCompiler.trie_ftable tries : forwarding_table) R) = [].
-Proof.
-  unfold dest_edges.
-  induction tries as [|t tries IH];
-    cbn [DistributedDatalogToHardwareCompiler.trie_ftable fold_right].
-  - unfold get_or_default, get_or. rewrite map.get_empty. reflexivity.
-  - rewrite mupd_with_default_eq_put, get_or_default_put. destr (eqb t.(trel) R).
-    + cbn [flat_map app]. exact IH.
-    + exact IH.
-Qed.
-
-Lemma trie_ftable_no_edges (tries : list trie) (R : rel_id) (ts : list destination) :
-  map.get (DistributedDatalogToHardwareCompiler.trie_ftable tries : forwarding_table) R = Some ts ->
-  dest_edges ts = [].
-Proof.
-  intros H. rewrite <- (get_or_default_Some _ _ _ H). apply trie_ftable_no_edges'.
-Qed.
-
-Lemma trie_ftables_no_edges (ninfos : list node_info) (n : node_id) (ftt : forwarding_table)
-    (R : rel_id) (ts : list destination) :
-  map.get (DistributedDatalogToHardwareCompiler.trie_ftables ninfos : node_ftable_map) n = Some ftt ->
-  map.get ftt R = Some ts ->
-  dest_edges ts = [].
-Proof.
-  unfold DistributedDatalogToHardwareCompiler.trie_ftables. revert ftt.
-  induction ninfos as [|ninfo ninfos IH]; cbn [List.map map.of_list]; intros ftt Hn HR.
-  - rewrite map.get_empty in Hn. discriminate.
-  - rewrite map.get_put_dec in Hn. destr (eqb ninfo.(nid) n).
-    + injection Hn as Hn. subst ftt. exact (trie_ftable_no_edges _ R ts HR).
-    + exact (IH ftt Hn HR).
-Qed.
-
-(* the computed table forwards [R] out of [n] to exactly the external table's next hops *)
-Lemma dest_edges_compute (ftables : internode_forwarding_tables) (ninfos : list node_info)
-    (n : node_id) (R : rel_id) :
-  dest_edges (node_rel_dests (compute_forwarding_table ftables ninfos) n R) = next_hops ftables n R.
-Proof.
-  unfold node_rel_dests, DistributedDatalogToHardwareCompiler.compute_forwarding_table,
-    get_or_default, get_or, DistributedDatalogToHardwareCompiler.edge_ftables.
-  rewrite union_with_get, get_map_values.
-  destruct (map.get ftables n) as [ft|] eqn:Hn;
-    destruct (map.get (DistributedDatalogToHardwareCompiler.trie_ftables ninfos) n)
-      as [ftt|] eqn:Hnt; cbn [option_map default map_default].
-  - rewrite union_with_get, get_map_values.
-    destruct (map.get ft R) as [hops|] eqn:HR;
-      destruct (map.get ftt R) as [ts|] eqn:HtR; cbn [option_map].
-    + rewrite dest_edges_app, dest_edges_map_edge, (trie_ftables_no_edges _ _ _ _ _ Hnt HtR).
-      apply app_nil_r.
-    + apply dest_edges_map_edge.
-    + rewrite (trie_ftables_no_edges _ _ _ _ _ Hnt HtR). reflexivity.
-    + reflexivity.
-  - rewrite get_map_values. destruct (map.get ft R) as [hops|] eqn:HR; cbn [option_map].
-    + apply dest_edges_map_edge.
-    + reflexivity.
-  - cbv [default map_default list_default]. rewrite map.get_empty.
-    destruct (map.get ftt R) as [ts|] eqn:HtR.
-    + rewrite (trie_ftables_no_edges _ _ _ _ _ Hnt HtR). reflexivity.
-    + reflexivity.
-  - cbv [default map_default list_default]. rewrite !map.get_empty. reflexivity.
-Qed.
-
-Lemma has_fwd_edge_compute (ftables : internode_forwarding_tables) (ninfos : list node_info)
-    (n : node_id) (R : rel_id) (m : node_id) :
-  has_fwd_edge (compute_forwarding_table ftables ninfos) n R m <-> In m (next_hops ftables n R).
-Proof. unfold has_fwd_edge. rewrite dest_edges_compute. reflexivity. Qed.
-
 (* an edge of the graph the table induces for [R] is exactly a recorded next hop *)
-Lemma cg_edge_graph_of_ftables (ftables : internode_forwarding_tables) (R : rel_id) (n m : node_id) :
-  cg_edge (graph_of_ftables_at_rel ftables R) n m <-> In m (next_hops ftables n R).
+Lemma cg_edge_graph_of_ftables (ftables : node_ftable_map) (R : rel_id) (n m : node_id) :
+  cg_edge (graph_of_ftables_at_rel ftables R) n m <-> has_fwd_edge ftables n R m.
 Proof.
   unfold ComputableGraph.cg_edge, ComputableGraph.check_edge_exists,
     DistributedDatalogToHardwareCompiler.graph_of_ftables_at_rel,
-    DistributedDatalogToHardwareCompiler.edges_of_ftables_at_rel, get_or_default, get_or.
+    DistributedDatalogToHardwareCompiler.edges_of_ftables_at_rel,
+    has_fwd_edge, node_rel_dests, get_or_default, get_or.
   cbn [ComputableGraph.edges]. rewrite get_map_values.
   destruct (map.get ftables n) as [ft|] eqn:Hn; cbn [option_map].
   - rewrite <- get_node_set_of_list.
@@ -191,13 +84,11 @@ Qed.
 
 (* the decidable check on an externally generated table gives exactly the edge-soundness the
    forwarding proofs used to get from [get_path_spec]. *)
-Lemma ftables_in_graphb_sound (g : node_graph) (ftables : internode_forwarding_tables)
-    (ninfos : list node_info) :
-  ftables_in_graphb g ftables = true ->
-  ftable_edges_sound g (compute_forwarding_table ftables ninfos).
+Lemma ftables_in_graphb_sound (g : node_graph) (ftables : node_ftable_map) :
+  ftables_in_graphb g ftables = true -> ftable_edges_sound g ftables.
 Proof.
-  intros Hcheck node rel m Hfwd. apply has_fwd_edge_compute in Hfwd.
-  unfold get_or_default, get_or in Hfwd.
+  intros Hcheck node rel m Hfwd.
+  unfold has_fwd_edge, node_rel_dests, get_or_default, get_or in Hfwd.
   destruct (map.get ftables node) as [ft|] eqn:Hnode;
     [| cbv [default map_default list_default] in Hfwd; rewrite map.get_empty in Hfwd; destruct Hfwd].
   pose proof (map.get_forallb _ ftables Hcheck node ft Hnode) as Hft.
